Ragequit for today

src/partie3.v
@@ -4,17 +4,17 @@ Load partie2.
 (* Question 2 *)
 Inductive Instruction :=
     | Access : nat -> Instruction
-    | Grab : Instruction
-    | Push : (list Instruction) -> Instruction
+    | Grab : Instruction -> Instruction
+    | Push : Instruction -> Instruction -> Instruction
 .
 Inductive Stack_type : Type := 
     | Nil : Stack_type
-    | Stack : ((list Instruction) * Stack_type) -> Stack_type -> Stack_type
+    | Stack : (Instruction * Stack_type) -> Stack_type -> Stack_type
 .
 
 Definition Environment : Type := Stack_type.
 
-Definition State : Type := ((list Instruction) * Environment * Stack_type).
+Definition State : Type := (Instruction * Environment * Stack_type).
 
 Inductive StateOption :=
     | None : StateOption
@@ -24,11 +24,17 @@ Inductive StateOption :=
 (* Question 3 *)
 Definition step_kirvine (state: State) : StateOption :=
     match state with
-    | ((Access 0) :: _, Stack (c0, e0) _, s) => Some ((c0, e0, s))
-    | ((Access (S n)) :: c, Stack (_, _) e, s) => Some (((Access n) :: c, e, s))
-    | ((Push cp) :: c, e, s) => Some ((c, e, Stack (cp, e) s))
-    | (Grab :: c, e, Stack (c0, e0) s) => Some (c, Stack (c0, e0) e, s)
+    | ((Access 0), Stack (c0, e0) _, s) => Some ((c0, e0, s))
+    | ((Access (S n)), Stack (_, _) e, s) => Some (((Access n), e, s))
+    | ((Push cp c), e, s) => Some ((c, e, Stack (cp, e) s))
+    | (Grab c, e, Stack (c0, e0) s) => Some (c, Stack (c0, e0) e, s)
     | _ => None
     end
 .
 
+Definition is_state (s: StateOption) :=
+    match s with
+    | None => False
+    | Some _ => True
+    end
+.
