src/partie4.v
@@ -1,12 +1,15 @@
 Add LoadPath "." as CoqDirectory.
 Load partie3.
 
-Fixpoint Comp (t: DeBruijn) : list Instruction :=
+Fixpoint Comp (t: DeBruijn) : Instruction :=
     match t with
-    | Lambda t => Grab :: (Comp t)
-    | Application tp1 tp2 => (Push (Comp tp1)) :: (Comp tp2)
-    | Var n => (Access n) :: []
+    | Lambda t => Grab (Comp t)
+    | Application tp1 tp2 => (Push (Comp tp1) (Comp tp2))
+    | Var n => (Access n)
     | Protect tp => Comp tp
     end
 .
 
+Definition CompState (t: DeBruijn) : State :=
+    (Comp t, Nil, Nil)
+.
