src/partie5.v
@@ -1,2 +1,123 @@
 Add LoadPath "." as CoqDirectory.
 Load partie4.
+
+Fixpoint tau_code (t: Instruction) : DeBruijn :=
+    match t with
+    | (Access n)=> Var n
+    | (Push cp c) => Application (tau_code cp) (tau_code c)
+    | Grab c => Lambda (tau_code c)
+    end
+.
+(* τ((c0,e0).e)  =  [0←τ(c0)[0←τ(e0)],u1...un]oùτ(e) = [0←u1...un] *)
+
+Fixpoint tau_environment_aux (e: Environment) : list DeBruijn :=
+    match e with 
+    | Stack (c_0, e_0) e_suite => 
+        ((tau_code(c_0))[0 <-- (tau_environment_aux e_0)]) :: (tau_environment_aux e_suite)
+    | Nil => []
+    end 
+.
+
+Definition tau_environment : Environment -> DeBruijn -> DeBruijn :=
+    fun e t => t[0 <-- (tau_environment_aux e)]
+.
+
+Fixpoint tau_aux (c: Instruction) (e: Environment) (s: Stack_type) : DeBruijn :=
+    match s with
+    | Stack (c_0, e_0) s_suite =>
+        Application (tau_environment e (tau_code c)) (tau_aux c_0 e_0 s_suite)
+    | Nil => tau_environment e (tau_code c)
+    end
+.
+
+Definition tau : State -> DeBruijn :=
+    (fun '(c, e, s) => tau_aux c e s)
+.
+
+Lemma protected_tau :
+    forall (c: Instruction), S(tau_code c)
+.
+Proof.
+    intro c.
+    induction c.
+    intuition.
+    intuition.
+    intuition.
+    unfold tau_code in H. simpl in H. intuition.
+Qed.
+
+Theorem tau_comp_identity :
+    forall (t: DeBruijn), tau (CompState t) = tau_code (Comp t)
+.
+Proof.
+    intro t.
+    induction t.
+    trivial.
+    simpl. unfold tau_environment.
+    simpl. assert (S(tau_code (Comp t))). apply (protected_tau (Comp t)).
+    rewrite safe_deprotect. exact H.
+    reflexivity. simpl. 
+    unfold tau_environment.
+    assert (tau_environment_aux Nil = []). auto.
+    rewrite H. rewrite (substitution_multiple_nil). 
+    assert (S(tau_code (Comp t1))). apply (protected_tau (Comp t1)).
+    assert (S(tau_code (Comp t2))). apply (protected_tau (Comp t2)).
+    assert (S(tau_code (Comp t1)) /\ S(tau_code (Comp t2))). intuition.
+    unfold protected. intuition. reflexivity.
+    simpl. unfold tau_environment.
+    intuition.
+Qed.
+
+Print substitution_multiple_commut.
+
+Fixpoint stack_length (e: Environment) :=
+    match e with
+    | Nil => 0
+    | Stack a suite => 1 + (stack_length suite)
+    end 
+.
+
+Inductive correct_stack : Stack_type -> Prop :=
+    | nil_correct : correct_stack Nil
+    | correct_trans : forall (c_0: Instruction),
+        forall (e_0: Environment), forall (e: Environment),
+        (C[stack_length e_0](tau_code(c_0))) -> 
+        correct_stack e_0 -> correct_stack e -> correct_stack (Stack (c_0, e_0) e)
+.
+
+Definition correct_state : State -> Prop :=
+    fun '(c, e, s) => correct_stack (Stack (c, e) s)
+.
+
+Notation "CoS( s )" := (correct_state s).
+
+Definition correct_option_state (t: StateOption) :=
+    match t with
+    | None => False
+    | Some s => CoS(s)
+    end
+.
+
+Notation "CoSo( s )" := (correct_option_state(s)).
+
+Theorem correct_state_trans : forall (s1: State), forall (s2: State),
+    CoS(s1) -> step_kirvine s1 = Some s2 -> CoS(s2)
+.
+Proof.
+    move => s1 s2 CoS_s1 s1_s2_rel.
+    induction s1.
+    destruct a.
+    unfold correct_state.
+    unfold correct_state in CoS_s1.
+    destruct s2. destruct p.
+    pose (s1 := Stack(i, e) b).
+    fold s1 in CoS_s1.
+    induction s1.
+    apply correct_trans.
+    destruct step_kirvine in s1_s2_rel.
+    contradict s1_s2_rel. intuition.
+    
+
+    
+
+    
